Propagate more CPUID preconditions through call graph

providers/evercrypt/fst/EverCrypt.AutoConfig2.fst
@@ -69,7 +69,7 @@ let wants_hacl () = B.recall user_wants_hacl; B.index user_wants_hacl 0ul
 let wants_openssl () = B.recall user_wants_openssl; B.index user_wants_openssl 0ul
 let wants_bcrypt () = B.recall user_wants_bcrypt; B.index user_wants_bcrypt 0ul
 
-let fp () =
+let fp_cpu_flags () =
   B.loc_buffer cpu_has_shaext `B.loc_union`
   B.loc_buffer cpu_has_aesni `B.loc_union`
   B.loc_buffer cpu_has_pclmulqdq `B.loc_union`
@@ -78,7 +78,10 @@ let fp () =
   B.loc_buffer cpu_has_bmi2 `B.loc_union`
   B.loc_buffer cpu_has_adx `B.loc_union`
   B.loc_buffer cpu_has_sse `B.loc_union`
-  B.loc_buffer cpu_has_movbe `B.loc_union`
+  B.loc_buffer cpu_has_movbe
+
+let fp () =
+  fp_cpu_flags() `B.loc_union`
   B.loc_buffer user_wants_hacl `B.loc_union`
   B.loc_buffer user_wants_vale `B.loc_union`
   B.loc_buffer user_wants_openssl `B.loc_union`
@@ -99,7 +102,7 @@ let recall () =
   B.recall user_wants_openssl;
   B.recall user_wants_bcrypt
 
-#set-options "--z3rlimit 50"
+#set-options "--z3rlimit 400"
 let init () =
   // TODO: use an && here once macros are improved
   let h0 = ST.get () in
@@ -128,10 +131,20 @@ let init () =
         B.upd cpu_has_bmi2 0ul true;
         B.recall cpu_has_adx;
         B.upd cpu_has_adx 0ul true
+      end;
+      if Vale.Wrapper.X64.Cpuid.check_sse () <> 0UL then begin
+        B.recall cpu_has_sse;
+        B.upd cpu_has_sse 0ul true
+      end;
+      if Vale.Wrapper.X64.Cpuid.check_movbe () <> 0UL then begin
+        B.recall cpu_has_movbe;
+        B.upd cpu_has_movbe 0ul true
       end
     end;
   let h1 = ST.get () in
-  assert (B.modifies (fp ()) h0 h1);
+  assert (B.modifies (fp_cpu_flags ()) h0 h1);
+  assert (B.loc_includes (fp ()) (fp_cpu_flags()));
+  assert (B.modifies (fp()) h0 h1);
   B.recall user_wants_hacl;
   B.upd user_wants_hacl 0ul SC.hacl;
   B.recall user_wants_vale;
